paxos/proof_agreement.dfy
@@ -22,21 +22,6 @@ lemma InitImpliesAgreementChosenInv(c:Constants, ds:DistrSys)
 {}
 
 
-/* Agreement_Chosen_Inv && Next ==> Agreement_Chosen_Inv' */
-lemma NextPreservesAgreementInv(c:Constants, ds:DistrSys, ds':DistrSys) 
-    requires Agreement_Chosen_Inv(c, ds)
-    requires Next(c, ds, ds')
-    ensures Agreement_Chosen_Inv(c, ds')
-{
-    NextPreservesTrivialities(c, ds, ds');
-    if SomeLeaderHasDecided(c, ds) {
-        NextPreservesAgreementInv_SomeoneHadDecided(c, ds, ds');
-    } else {
-        NextPreservesAgreementInv_NoneHadDecided(c, ds, ds');
-    }
-}
-
-
 lemma NextPreservesTrivialities(c:Constants, ds:DistrSys, ds':DistrSys) 
     requires Agreement_Chosen_Inv(c, ds)
     requires Next(c, ds, ds')
@@ -51,239 +36,324 @@ lemma NextPreservesTrivialities(c:Constants, ds:DistrSys, ds':DistrSys)
 }
 
 
-//////////////           Agreement Sub-Lemma: Existing decision            ///////////////
-
-
-lemma NextPreservesAgreementInv_SomeoneHadDecided(c:Constants, ds:DistrSys, ds':DistrSys) 
+/* Agreement_Chosen_Inv && Next ==> Agreement_Chosen_Inv' */
+lemma NextPreservesAgreementChosenInv(c:Constants, ds:DistrSys, ds':DistrSys) 
     requires Agreement_Chosen_Inv(c, ds)
     requires Next(c, ds, ds')
-    requires SomeLeaderHasDecided(c, ds)
-    ensures SomeLeaderHasDecided(c, ds')
     ensures Agreement_Chosen_Inv(c, ds')
 {
     NextPreservesTrivialities(c, ds, ds');
-    var actor, recvIos, sendIos :| PaxosNextOneAgent(c, ds, ds', actor, recvIos, sendIos);
-    if actor.agt == Ldr {
-        NextPreservesAgreementInv_SomeoneHadDecided_LeaderAction(c, ds, ds', actor, recvIos, sendIos);
-    } else {
-        NextPreservesAgreementInv_SomeoneHadDecided_AcceptorAction(c, ds, ds', actor, recvIos, sendIos);
-    }
-}
-
-
-lemma {:timeLimitMultiplier 2} NextPreservesAgreementInv_SomeoneHadDecided_AcceptorAction(c:Constants, ds:DistrSys, ds':DistrSys, actor:Id, recvIos:seq<Packet>, sendIos:seq<Packet>) 
-    requires Agreement_Chosen_Inv(c, ds)
-    requires Next(c, ds, ds')
-    requires ds'.WF(c) && Trivialities(c, ds')
-    requires SomeLeaderHasDecided(c, ds)
-    requires PaxosNextOneAgent(c, ds, ds', actor, recvIos, sendIos)
-    requires actor.agt == Acc
-    ensures SomeLeaderHasDecided(c, ds')
-    ensures Agreement_Chosen_Inv(c, ds')
-{
-    NextPreservesAgreementInv_SomeoneHadDecided_AcceptorAction_PromisedImpliesNoMoreAccepts(c, ds, ds', actor, recvIos, sendIos);
-    
-    // Prove Agreement_Inv_Decided properties
-    forall i2 | c.ValidLdrIdx(i2) && LeaderHasDecided(c, ds', i2) 
-    ensures Agreement_Inv_Decided(c, ds', i2)
-    {
-        // Note i2 has been decided in ds; it's not a new decision
-        assert LeaderHasDecided(c, ds, i2); 
-        var b2, v2 := ds.leaders[i2].ballot, ds.leaders[i2].val;
-
-        // Proving LargerBallotsPromiseQrms(c, ds', v2, b2);
-        forall b' | BalLt(b2, b') 
-        ensures LargerBalQuorumHasSeenB(c, ds', b2, b')
-        {
-            forall qrm:set<Packet> | QuorumOfPromiseMsgs(c, ds', qrm, b') 
-            ensures QuorumHasSeenB(c, ds', qrm, b2)
-            {
-                // Proof by contradiction. Suppose false. Then f+1 acceptors promised
-                // b' without accepting b2. Then by PromisedImpliesNoMoreAccepts, there
-                // is no quorum of Accept(b2), and (b2) cannot be decided. 
-                if (exists prom_qrm :: 
-                        && QuorumOfPromiseMsgs(c, ds', prom_qrm, b')
-                        && !QuorumHasSeenB(c, ds', prom_qrm, b2)
-                ){
-                    var prom_qrm :| 
-                        && QuorumOfPromiseMsgs(c, ds', prom_qrm, b') 
-                        && !QuorumHasSeenB(c, ds', prom_qrm, b2);
-                    // Now prove that the corresponding acceptors did not accept (b2, v2)
-                    assert PromisedImpliesNoMoreAccepts(c, ds');
-                    forall acc_p | 
-                            && acc_p in ds'.network.sentPackets 
-                            && (exists prom_p : Packet :: prom_p in prom_qrm && acc_p.src == prom_p.src)
-                            && acc_p.msg.Accept?
-                    ensures acc_p.msg.bal != b2
-                    {}
-                    forall acc_set : set<Packet> | 
-                            && UniqueSources(acc_set)
-                            && (forall p | p in acc_set :: p.msg.Accept?)
-                            && (forall p | p in acc_set :: p.msg.bal == b2)
-                            && (forall p | p in acc_set :: p in ds'.network.sentPackets)
-                    ensures |acc_set| < c.f + 1
-                    {
-                        if |acc_set| >= c.f + 1 {
-                            assert QuorumOfAcceptMsgs(c, ds', acc_set, b2);
-                            var _ := lemma_QuorumIntersection(c, ds', prom_qrm, b', acc_set, b2);
-                            assert false;
-                        }
-                    }
-                    Lemma_DecidedImpliesQuorumOfAccepts(c, ds', i2);
-                    assert false;
-                }
-            }
-        }
-        assert LargerBallotsPromiseQrms(c, ds', b2);
-    }
-}
-
-
-lemma NextPreservesAgreementInv_SomeoneHadDecided_AcceptorAction_PromisedImpliesNoMoreAccepts(c:Constants, ds:DistrSys, ds':DistrSys, actor:Id, recvIos:seq<Packet>, sendIos:seq<Packet>) 
-    requires Agreement_Chosen_Inv(c, ds)
-    requires Next(c, ds, ds')
-    requires ds'.WF(c)
-    requires Trivialities(c, ds')
-    requires SomeLeaderHasDecided(c, ds)
-    requires PaxosNextOneAgent(c, ds, ds', actor, recvIos, sendIos)
-    requires actor.agt == Acc
-    ensures SomeLeaderHasDecided(c, ds')
-    ensures PromisedImpliesNoMoreAccepts(c, ds')
-{}
-
-
-lemma NextPreservesAgreementInv_SomeoneHadDecided_LeaderAction(c:Constants, ds:DistrSys, ds':DistrSys, actor:Id, recvIos:seq<Packet>, sendIos:seq<Packet>) 
-    requires Agreement_Chosen_Inv(c, ds)
-    requires Next(c, ds, ds')
-    requires ds'.WF(c) && Trivialities(c, ds')
-    requires SomeLeaderHasDecided(c, ds)
-    requires PaxosNextOneAgent(c, ds, ds', actor, recvIos, sendIos)
-    requires actor.agt == Ldr
-    ensures SomeLeaderHasDecided(c, ds')
-    ensures Agreement_Chosen_Inv(c, ds')
-{
-    var i1 :| c.ValidLdrIdx(i1) && LeaderHasDecided(c, ds, i1);
-    var b1, v1 := ds.leaders[i1].ballot, ds.leaders[i1].val;
-
-    forall i | c.ValidLdrIdx(i) && LeaderHasDecided(c, ds', i) 
-    ensures Agreement_Inv_Decided(c, ds', i)
-    {
-         // TODO
+    if SomeValueChosen(c, ds) {
+        // TODO
         assume false;
-        var b, v := ds'.leaders[i].ballot, ds'.leaders[i].val;
-        assert LargerBallotPhase2LeadersV(c, ds', v, b);
-        assert LargerBallotAcceptors(c, ds', v, b);     // Trivial
-        assert LargerBallotPromiseMsgs(c, ds', v, b);   // Trivial
-        assert LargerBallotProposeMsgs(c, ds', v, b);   // Trivial
-        assert LargerBallotsPromiseQrms(c, ds', b);
-        assert LeaderHasQuorumOfAccepts(c, ds', i);
+    } else {
+        // TODO
+        AgreementChosenInv_NoneChosen(c, ds, ds');
     }
-    NextPreservesAgreementInv_SomeoneHadDecided_LeaderAction_Agreement(c, ds, ds', actor, recvIos, sendIos);
-    assert Trivialities(c, ds');
-    assert LdrAcceptsSetCorrespondToAcceptMsg(c, ds');
-    assert LdrPromisesSetCorrespondToPromiseMsg(c, ds');
-    assert AccPromisedBallotLargerThanAccepted(c, ds');
-    assert AcceptMsgImpliesAccepted(c, ds');
-    assert PromisedImpliesNoMoreAccepts(c, ds');
-    assert Agreement_Chosen_Inv(c, ds');
 }
 
+// //////////////          Agreement Sub-Lemma: No existing decision          ///////////////
 
-lemma NextPreservesAgreementInv_SomeoneHadDecided_LeaderAction_Agreement(c:Constants, ds:DistrSys, ds':DistrSys, actor:Id, recvIos:seq<Packet>, sendIos:seq<Packet>) 
+
+lemma AgreementChosenInv_NoneChosen(c:Constants, ds:DistrSys, ds':DistrSys) 
     requires Agreement_Chosen_Inv(c, ds)
-    requires Next(c, ds, ds')
     requires ds'.WF(c) && Trivialities(c, ds')
-    requires SomeLeaderHasDecided(c, ds)
-    requires PaxosNextOneAgent(c, ds, ds', actor, recvIos, sendIos)
-    requires actor.agt == Ldr
-    ensures SomeLeaderHasDecided(c, ds')
-    ensures Agreement(c, ds')
-{
-    var i1 :| c.ValidLdrIdx(i1) && LeaderHasDecided(c, ds, i1);
-    var b1, v1 := ds.leaders[i1].ballot, ds.leaders[i1].val;
-
-    forall i2 | i2 != i1 && c.ValidLdrIdx(i2) && LeaderHasDecided(c, ds', i2) 
-    ensures TwoLeadersHaveSameV(c, ds', i1, i2) 
-    {
-        var b2, v2 := ds.leaders[i2].ballot, ds.leaders[i2].val;
-        if actor.agt == Ldr {
-            if actor.idx == i2 {
-                if !LeaderHasDecided(c, ds, i2) {
-                    // This is where the heavy lifting is
-                    assert LeaderInPhase2(c, ds, i2);
-                    if BalLtEq(b1, b2) {
-                        assert LeaderHasValueV(c, ds, i2, v1);
-                        assert LeaderHasValueV(c, ds', i2, v1);
-                    } else {
-                        // TODO
-                        assume false;
-
-                        assert LargerBallotPhase2LeadersV(c, ds', v2, b2);
-                        assert BalLtEq(b2, b1);
-                        assert LeaderHasValueV(c, ds', i1, v2);
-                    }
-                } else {
-                    assert TwoLeadersHaveSameV(c, ds', i1, i2);
-                }
-            } else {
-                assert LeaderHasDecided(c, ds, i2);
-                assert TwoLeadersHaveSameV(c, ds', i1, i2);
-            }
-        } else { 
-            assert TwoLeadersHaveSameV(c, ds', i1, i2);
-        }
-    }
-    assert Agreement(c, ds');   
-}
-
-
-
-
-
-
-
-
-//////////////          Agreement Sub-Lemma: No existing decision          ///////////////
-
-
-lemma NextPreservesAgreementInv_NoneHadDecided(c:Constants, ds:DistrSys, ds':DistrSys) 
-    requires Agreement_Chosen_Inv(c, ds)
     requires Next(c, ds, ds')
-    requires !SomeLeaderHasDecided(c, ds)
+    requires !SomeValueChosen(c, ds)
     ensures Agreement_Chosen_Inv(c, ds')
 {
     var actor, recvIos:seq<Packet>, sendIos :| PaxosNextOneAgent(c, ds, ds', actor, recvIos, sendIos);
     if actor.agt == Ldr {
         // If actor is a Leader
-        assert Agreement(c, ds');
-        assert LdrBallotNotBottom(c, ds');
-        assert LdrAcceptsSetCorrespondToAcceptMsg(c, ds');
-        assert LdrPromisesSetCorrespondToPromiseMsg(c, ds');
-        assert AccPromisedBallotLargerThanAccepted(c, ds'); 
-        assert AcceptMsgImpliesAccepted(c, ds');
-        assert PromisedImpliesNoMoreAccepts(c, ds');
-        assert Trivialities(c, ds');
-        
-        // Prove Agreement_Inv_Decided properties
-        forall i2 | c.ValidLdrIdx(i2) && LeaderHasDecided(c, ds', i2) 
-        ensures Agreement_Inv_Decided(c, ds', i2)
-        {
-            // TODO:
-            assume false;
-            var b2, v2 := ds.leaders[i2].ballot, ds.leaders[i2].val;
-            assert LargerBallotPhase2LeadersV(c, ds, v2, b2);
-            assert LargerBallotAcceptors(c, ds', v2, b2);
-            assert LargerBallotPromiseMsgs(c, ds', v2, b2);
-            assert LargerBallotProposeMsgs(c, ds', v2, b2);
-            assert LeaderHasQuorumOfAccepts(c, ds', i2);
-            assert LargerBallotsPromiseQrms(c, ds', b2);
-        }
-        assert Agreement_Chosen_Inv(c, ds');
-    } else {
-        // If actor is an Acceptor
-        // This case should be trivial
         assume false;
         assert Agreement_Chosen_Inv(c, ds');
+    } else {
+        // If actor is an Acceptor: This is the tricky case as 
+        // some value may be chosen in this step
+        AgreementChosenInv_NoneChosen_AccAction(c, ds, ds', actor, recvIos, sendIos);
     }
 }
+
+
+lemma AgreementChosenInv_NoneChosen_AccAction(
+c:Constants, ds:DistrSys, ds':DistrSys, actor:Id, recvIos:seq<Packet>, sendIos:seq<Packet>)
+    requires Agreement_Chosen_Inv(c, ds)
+    requires ds'.WF(c) && Trivialities(c, ds')
+    requires Next(c, ds, ds')
+    requires PaxosNextOneAgent(c, ds, ds', actor, recvIos, sendIos)
+    requires actor.agt == Acc
+    requires !SomeValueChosen(c, ds)
+    ensures Agreement_Chosen_Inv(c, ds')
+{
+    AgreementChosenInv_NoneChosen_AccAction_AgreementChosen(c, ds, ds', actor, recvIos, sendIos);
+
+    assume false;
+    assert OneValuePerBallot(c, ds');
+
+    // Leader state
+    assert LdrAcceptsSetCorrespondToAcceptMsg(c, ds');
+    assert LdrPromisesSetCorrespondToPromiseMsg(c, ds');
+
+    // Acceptor state
+    assert AccPromisedBallotLargerThanAccepted(c, ds');
+
+    // Messages
+    assert PromiseVBImpliesAcceptMsg(c, ds');
+    assert AcceptMsgImpliesAccepted(c, ds');
+    assert AcceptedImpliesAcceptMessage(c, ds');
+    assert AcceptMsgImpliesProposeMsg(c, ds');
+    assert ProposeMsgImpliesQuorumOfPromise(c, ds');
+    assert PromisedImpliesNoMoreAccepts(c, ds');
+
+    // Chosen
+    forall b, v | Chosen(c, ds', b, v) 
+    ensures Agreement_Chosen_Inv_SomeValChosen(c, ds', b, v)
+    {
+        assume false;
+        assert Agreement_Chosen_Inv_SomeValChosen(c, ds', b, v); //
+    }
+    assert Agreement_Chosen_Inv(c, ds');
+}
+
+
+
+lemma AgreementChosenInv_NoneChosen_AccAction_AgreementChosen(
+c:Constants, ds:DistrSys, ds':DistrSys, actor:Id, recvIos:seq<Packet>, sendIos:seq<Packet>)
+    requires Agreement_Chosen_Inv(c, ds)
+    requires ds'.WF(c) && Trivialities(c, ds')
+    requires Next(c, ds, ds')
+    requires PaxosNextOneAgent(c, ds, ds', actor, recvIos, sendIos)
+    requires actor.agt == Acc
+    requires !SomeValueChosen(c, ds)
+    ensures Agreement_Chosen(c, ds')
+{
+    // At most one value can be chosen in ds'.
+    if recvIos[0].msg.Propose? {
+        var a, a' := ds.acceptors[actor.idx], ds'.acceptors[actor.idx];
+        if BalLtEq(a.promised, recvIos[0].msg.bal) {
+            var b, v := recvIos[0].msg.bal, recvIos[0].msg.val;
+            forall b', v' | Chosen(c, ds', b', v') 
+            ensures b' == b && v' == v
+            {
+                if !(b' == b && v' == v) {
+                    assert Chosen(c, ds, b', v');
+                    assert false;
+                }
+            }
+        } else {
+            assert forall p:Packet | p in ds'.network.sentPackets && p.msg.Accept? :: p in ds.network.sentPackets;
+            if exists b, v :: Chosen(c, ds', b, v) { 
+                lemma_NoNewAcceptsImpliesNoNewChosen(c, ds, ds');
+                assert false;
+            }
+        }
+    } else {
+        // No new Accept packets generated in this step, so nothing is chosen in ds'
+        assert forall p:Packet | p in ds'.network.sentPackets && p.msg.Accept? :: p in ds.network.sentPackets;
+        if exists b, v :: Chosen(c, ds', b, v) { 
+            lemma_NoNewAcceptsImpliesNoNewChosen(c, ds, ds');
+            assert false;
+        }
+    }
+}
+
+
+
+
+
+
+
+
+
+
+
+
+
+
+//////////////           Agreement Sub-Lemma: Existing decision            ///////////////
+
+
+// lemma NextPreservesAgreementInv_SomeoneHadDecided(c:Constants, ds:DistrSys, ds':DistrSys) 
+//     requires Agreement_Chosen_Inv(c, ds)
+//     requires Next(c, ds, ds')
+//     requires SomeLeaderHasDecided(c, ds)
+//     ensures SomeLeaderHasDecided(c, ds')
+//     ensures Agreement_Chosen_Inv(c, ds')
+// {
+//     NextPreservesTrivialities(c, ds, ds');
+//     var actor, recvIos, sendIos :| PaxosNextOneAgent(c, ds, ds', actor, recvIos, sendIos);
+//     if actor.agt == Ldr {
+//         NextPreservesAgreementInv_SomeoneHadDecided_LeaderAction(c, ds, ds', actor, recvIos, sendIos);
+//     } else {
+//         NextPreservesAgreementInv_SomeoneHadDecided_AcceptorAction(c, ds, ds', actor, recvIos, sendIos);
+//     }
+// }
+
+
+// lemma {:timeLimitMultiplier 2} NextPreservesAgreementInv_SomeoneHadDecided_AcceptorAction(c:Constants, ds:DistrSys, ds':DistrSys, actor:Id, recvIos:seq<Packet>, sendIos:seq<Packet>) 
+//     requires Agreement_Chosen_Inv(c, ds)
+//     requires Next(c, ds, ds')
+//     requires ds'.WF(c) && Trivialities(c, ds')
+//     requires SomeLeaderHasDecided(c, ds)
+//     requires PaxosNextOneAgent(c, ds, ds', actor, recvIos, sendIos)
+//     requires actor.agt == Acc
+//     ensures SomeLeaderHasDecided(c, ds')
+//     ensures Agreement_Chosen_Inv(c, ds')
+// {
+//     NextPreservesAgreementInv_SomeoneHadDecided_AcceptorAction_PromisedImpliesNoMoreAccepts(c, ds, ds', actor, recvIos, sendIos);
+    
+//     // Prove Agreement_Inv_Decided properties
+//     forall i2 | c.ValidLdrIdx(i2) && LeaderHasDecided(c, ds', i2) 
+//     ensures Agreement_Inv_Decided(c, ds', i2)
+//     {
+//         // Note i2 has been decided in ds; it's not a new decision
+//         assert LeaderHasDecided(c, ds, i2); 
+//         var b2, v2 := ds.leaders[i2].ballot, ds.leaders[i2].val;
+
+//         // Proving LargerBallotsPromiseQrms(c, ds', v2, b2);
+//         forall b' | BalLt(b2, b') 
+//         ensures LargerBalQuorumHasSeenB(c, ds', b2, b')
+//         {
+//             forall qrm:set<Packet> | QuorumOfPromiseMsgs(c, ds', qrm, b') 
+//             ensures QuorumHasSeenB(c, ds', qrm, b2)
+//             {
+//                 // Proof by contradiction. Suppose false. Then f+1 acceptors promised
+//                 // b' without accepting b2. Then by PromisedImpliesNoMoreAccepts, there
+//                 // is no quorum of Accept(b2), and (b2) cannot be decided. 
+//                 if (exists prom_qrm :: 
+//                         && QuorumOfPromiseMsgs(c, ds', prom_qrm, b')
+//                         && !QuorumHasSeenB(c, ds', prom_qrm, b2)
+//                 ){
+//                     var prom_qrm :| 
+//                         && QuorumOfPromiseMsgs(c, ds', prom_qrm, b') 
+//                         && !QuorumHasSeenB(c, ds', prom_qrm, b2);
+//                     // Now prove that the corresponding acceptors did not accept (b2, v2)
+//                     assert PromisedImpliesNoMoreAccepts(c, ds');
+//                     forall acc_p | 
+//                             && acc_p in ds'.network.sentPackets 
+//                             && (exists prom_p : Packet :: prom_p in prom_qrm && acc_p.src == prom_p.src)
+//                             && acc_p.msg.Accept?
+//                     ensures acc_p.msg.bal != b2
+//                     {}
+//                     forall acc_set : set<Packet> | 
+//                             && UniqueSources(acc_set)
+//                             && (forall p | p in acc_set :: p.msg.Accept?)
+//                             && (forall p | p in acc_set :: p.msg.bal == b2)
+//                             && (forall p | p in acc_set :: p in ds'.network.sentPackets)
+//                     ensures |acc_set| < c.f + 1
+//                     {
+//                         if |acc_set| >= c.f + 1 {
+//                             assert QuorumOfAcceptMsgs(c, ds', acc_set, b2);
+//                             var _ := lemma_QuorumIntersection(c, ds', prom_qrm, b', acc_set, b2);
+//                             assert false;
+//                         }
+//                     }
+//                     Lemma_DecidedImpliesQuorumOfAccepts(c, ds', i2);
+//                     assert false;
+//                 }
+//             }
+//         }
+//         assert LargerBallotsPromiseQrms(c, ds', b2);
+//     }
+// }
+
+
+// lemma NextPreservesAgreementInv_SomeoneHadDecided_AcceptorAction_PromisedImpliesNoMoreAccepts(c:Constants, ds:DistrSys, ds':DistrSys, actor:Id, recvIos:seq<Packet>, sendIos:seq<Packet>) 
+//     requires Agreement_Chosen_Inv(c, ds)
+//     requires Next(c, ds, ds')
+//     requires ds'.WF(c)
+//     requires Trivialities(c, ds')
+//     requires SomeLeaderHasDecided(c, ds)
+//     requires PaxosNextOneAgent(c, ds, ds', actor, recvIos, sendIos)
+//     requires actor.agt == Acc
+//     ensures SomeLeaderHasDecided(c, ds')
+//     ensures PromisedImpliesNoMoreAccepts(c, ds')
+// {}
+
+
+// lemma NextPreservesAgreementInv_SomeoneHadDecided_LeaderAction(c:Constants, ds:DistrSys, ds':DistrSys, actor:Id, recvIos:seq<Packet>, sendIos:seq<Packet>) 
+//     requires Agreement_Chosen_Inv(c, ds)
+//     requires Next(c, ds, ds')
+//     requires ds'.WF(c) && Trivialities(c, ds')
+//     requires SomeLeaderHasDecided(c, ds)
+//     requires PaxosNextOneAgent(c, ds, ds', actor, recvIos, sendIos)
+//     requires actor.agt == Ldr
+//     ensures SomeLeaderHasDecided(c, ds')
+//     ensures Agreement_Chosen_Inv(c, ds')
+// {
+//     var i1 :| c.ValidLdrIdx(i1) && LeaderHasDecided(c, ds, i1);
+//     var b1, v1 := ds.leaders[i1].ballot, ds.leaders[i1].val;
+
+//     forall i | c.ValidLdrIdx(i) && LeaderHasDecided(c, ds', i) 
+//     ensures Agreement_Inv_Decided(c, ds', i)
+//     {
+//          // TODO
+//         assume false;
+//         var b, v := ds'.leaders[i].ballot, ds'.leaders[i].val;
+//         assert LargerBallotPhase2LeadersV(c, ds', v, b);
+//         assert LargerBallotAcceptors(c, ds', v, b);     // Trivial
+//         assert LargerBallotPromiseMsgs(c, ds', v, b);   // Trivial
+//         assert LargerBallotProposeMsgs(c, ds', v, b);   // Trivial
+//         assert LargerBallotsPromiseQrms(c, ds', b);
+//         assert LeaderHasQuorumOfAccepts(c, ds', i);
+//     }
+//     NextPreservesAgreementInv_SomeoneHadDecided_LeaderAction_Agreement(c, ds, ds', actor, recvIos, sendIos);
+//     assert Trivialities(c, ds');
+//     assert LdrAcceptsSetCorrespondToAcceptMsg(c, ds');
+//     assert LdrPromisesSetCorrespondToPromiseMsg(c, ds');
+//     assert AccPromisedBallotLargerThanAccepted(c, ds');
+//     assert AcceptMsgImpliesAccepted(c, ds');
+//     assert PromisedImpliesNoMoreAccepts(c, ds');
+//     assert Agreement_Chosen_Inv(c, ds');
+// }
+
+
+// lemma NextPreservesAgreementInv_SomeoneHadDecided_LeaderAction_Agreement(c:Constants, ds:DistrSys, ds':DistrSys, actor:Id, recvIos:seq<Packet>, sendIos:seq<Packet>) 
+//     requires Agreement_Chosen_Inv(c, ds)
+//     requires Next(c, ds, ds')
+//     requires ds'.WF(c) && Trivialities(c, ds')
+//     requires SomeLeaderHasDecided(c, ds)
+//     requires PaxosNextOneAgent(c, ds, ds', actor, recvIos, sendIos)
+//     requires actor.agt == Ldr
+//     ensures SomeLeaderHasDecided(c, ds')
+//     ensures Agreement(c, ds')
+// {
+//     var i1 :| c.ValidLdrIdx(i1) && LeaderHasDecided(c, ds, i1);
+//     var b1, v1 := ds.leaders[i1].ballot, ds.leaders[i1].val;
+
+//     forall i2 | i2 != i1 && c.ValidLdrIdx(i2) && LeaderHasDecided(c, ds', i2) 
+//     ensures TwoLeadersHaveSameV(c, ds', i1, i2) 
+//     {
+//         var b2, v2 := ds.leaders[i2].ballot, ds.leaders[i2].val;
+//         if actor.agt == Ldr {
+//             if actor.idx == i2 {
+//                 if !LeaderHasDecided(c, ds, i2) {
+//                     // This is where the heavy lifting is
+//                     assert LeaderInPhase2(c, ds, i2);
+//                     if BalLtEq(b1, b2) {
+//                         assert LeaderHasValueV(c, ds, i2, v1);
+//                         assert LeaderHasValueV(c, ds', i2, v1);
+//                     } else {
+//                         // TODO
+//                         assume false;
+
+//                         assert LargerBallotPhase2LeadersV(c, ds', v2, b2);
+//                         assert BalLtEq(b2, b1);
+//                         assert LeaderHasValueV(c, ds', i1, v2);
+//                     }
+//                 } else {
+//                     assert TwoLeadersHaveSameV(c, ds', i1, i2);
+//                 }
+//             } else {
+//                 assert LeaderHasDecided(c, ds, i2);
+//                 assert TwoLeadersHaveSameV(c, ds', i1, i2);
+//             }
+//         } else { 
+//             assert TwoLeadersHaveSameV(c, ds', i1, i2);
+//         }
+//     }
+//     assert Agreement(c, ds');   
+// }
+
+
 }
